
\subsection{The chain rule, the product rule and the quotient rule}

\subsubsection{Chain rule}

\(f(x)=f(g(x))\)

\(\dfrac{\delta f}{\delta x}=\lim_{\epsilon \rightarrow 0^+}\dfrac{f(g(x+\epsilon) )-f(g(x))}{\epsilon }\)

\(\dfrac{\delta f}{\delta x}=\lim_{\epsilon \rightarrow 0^+}\dfrac{g(x+\epsilon )-g(x)}{g(x+\epsilon )-g(x)}\dfrac{f(g(x+\epsilon) )-f(g(x))}{\epsilon }\)

\(\dfrac{\delta f}{\delta x}=\lim_{\epsilon \rightarrow 0^+}\dfrac{g(x+\epsilon )-g(x)}{\epsilon }\dfrac{f(g(x+\epsilon) )-f(g(x))}{g(x+\epsilon )-g(x)}\)

\(\dfrac{\delta f}{\delta x}=\lim_{\epsilon \rightarrow 0^+}[\dfrac{g(x+\epsilon )-g(x)}{\epsilon }]\lim_{\epsilon \rightarrow 0^+}[\dfrac{f(g(x+\epsilon) )-f(g(x))}{g(x+\epsilon )-g(x)}]\)

\(\dfrac{\delta f}{\delta x}=\dfrac{\delta g}{\delta x}\dfrac{\delta f}{\delta g}\)

\subsubsection{Product rule}

\(y=f(x)g(x)\)

\(\dfrac{\delta y}{\delta x}=\lim_{\epsilon \rightarrow 0^+}\dfrac{f(x+\epsilon )g(x+\epsilon )-f(x)g(x)}{\epsilon }\)

\(\dfrac{\delta y}{\delta x}=\lim_{\epsilon \rightarrow 0^+}\dfrac{f(x+\epsilon )g(x+\epsilon )-f(x)g(x+\epsilon )+f(x)g(x+\epsilon )-f(x)g(x)}{\epsilon }\)

\(\dfrac{\delta y}{\delta x}=\lim_{\epsilon \rightarrow 0^+}\dfrac{f(x+\epsilon )g(x+\epsilon )-f(x)g(x+\epsilon )}{\epsilon }+\lim_{\epsilon \rightarrow 0^+}\dfrac{f(x)g(x+\epsilon )-f(x)g(x)}{\epsilon }\)

\(\dfrac{\delta y}{\delta x}=\lim_{\epsilon \rightarrow 0^+}g(x+\epsilon )\dfrac{f(x+\epsilon )-f(x)}{\epsilon }+\lim_{\epsilon \rightarrow 0^+}f(x)\dfrac{g(x+\epsilon )-g(x)}{\epsilon }\)

\(\dfrac{\delta y}{\delta x}=g(x)\dfrac{\delta f}{\delta x }+f(x)\dfrac{\delta g}{\delta x}\)

\subsubsection{Quotient rule}

\(y=\dfrac{f(x)}{g(x)}\)

\(\dfrac{\delta }{\delta x}y=\dfrac{\delta }{\delta x}\dfrac{f(x)}{g(x)}\)

\(\dfrac{\delta }{\delta x}y=\dfrac{\delta }{\delta x}f(x)\dfrac{1}{g(x)}\)

\(\dfrac{\delta }{\delta x}y=\dfrac{\delta f}{\delta x}\dfrac{1}{g(x)}-\dfrac{\delta g}{\delta x}\dfrac{f(x)}{g(x)^2}\)

\(\dfrac{\delta }{\delta x}y=\dfrac{\dfrac{\delta f}{\delta x}g(x)-\dfrac{\delta g}{\delta x}f(x)}{g(x)^2}\)

