
\subsection{Defining \(e\) as a binomial}

\subsubsection{Lemma}

\(f(n,i)=\frac{n!}{n^i(n-i)!}\)

\(f(n,i)=\frac{(n-i)!\prod_{j=n-i+1}^nj}{n^i(n-i)!}\)

\(f(n,i)=\frac{\prod_{j=n-i+1}^nj}{n^i}\)

\(f(n,i)=\frac{\prod_{j=1}^i(j+n-i)}{n^i}\)

\(f(n,i)=\prod_{j=1}^i\frac{j+n-i}{n}\)

\(f(n,i)=\prod_{j=1}^i(\frac{n}{n}+\frac{j-i}{n})\)

\(f(n,i)=\prod_{j=1}^i(1+\frac{j-i}{n})\)

\(\lim_{n\rightarrow \infty }f(n,i)=\lim_{n\rightarrow \infty }\prod_{j=1}^i(1+\frac{j-i}{n})\)

\(\lim_{n\rightarrow \infty }f(n,i)=\prod_{j=1}^i1\)

\(\lim_{n\rightarrow \infty }f(n,i)=1\)

\subsubsection{Defining \(e\)}

We know that:

\((a+b)^n=\sum^n_{i=0} a^i b^{n-i} \frac{n!}{i!(n-i)!}\)

Let's set \(b=1\)

\((a+1)^n=\sum^n_{i=0} a^i \frac{n!}{i!(n-i)!}\)

Let's set \(a=\frac{1}{n}\)

\((1+\frac{1}{n})^{n}=\sum^{n}_{i=0} \frac{1}{n^i} \frac{n!}{i!(n-i)!}\)

\((1+\frac{1}{n})^{n}=\sum^{n}_{i=0} \frac{1}{i!} \frac{n!}{n^i(n-i)!}\)

\(\lim_{n\rightarrow \infty }(1+\frac{1}{n})^{n}=\lim_{n\rightarrow \infty }\sum^{n}_{i=0} \frac{1}{i!} \frac{n!}{n^i(n-i)!}\)

From the lemma above:

\(\lim_{n\rightarrow \infty }(1+\frac{1}{n})^{n}=\sum^{\infty }_{i=0} \frac{1}{i!}\)

\(e=\sum^{\infty }_{i=0} \frac{1}{i!}\)

\subsubsection{Defining \(e^x\)}

\(e=\lim_{n\rightarrow \infty }(1+\frac{1}{n})^{n}\)

\(e^x=\lim_{n\rightarrow \infty }(1+\frac{1}{n})^{nx}\)

\(e^x=\lim_{n\rightarrow \infty }\sum^{nx}_{i=0} \frac{1}{n^i} \frac{(nx)!}{i!(nx-i)!}\)

\(e^x=\lim_{n\rightarrow \infty }\sum^{nx}_{i=0} \frac{x^i}{i!} \frac{(nx)!}{(nx)^i(nx-i)!}\)

From the lemma:

\(e^x=\sum^{\infty }_{i=0} \frac{x^i}{i!}\)

