\subsection{Addition of natural numbers}


\subsubsection{Definition}
Let’s add another function: addition. Defined by:

$\forall a \in \mathbb{N} (a+0=a)$

$\forall a b \in \mathbb{N} (a+s(b)=s(a+b))$

That is, adding zero to a number doesn’t change it, and \((a+b)+1=a+(b+1)\).

\subsubsection{Example}

Let’s use this to solve \(1+2\):

$1+2=1+s(1)$

$1+s(1)=s(1+1)$

$s(1+1)=s(1+s(0))$

$s(1+s(0))=s(s(1+0))$

$s(s(1+0))=s(s(1))$

$s(s(1))=s(2)$

$s(2)=3$

$1+2=3$

All addition can be done iteratively like this.

\subsubsection{Commutative property of addition}

Addition is commutative:

$x+y=y+x$

\subsubsection{Associative property of addition}

Addition is associative:

$x+(y+z)=(x+y)+z$

