
\subsection{The Lie bracket}

We can define the Lie bracket from the ring commutator.

We use the Lie bracket, rather than multiplication, as the operator over a field homomorphism.

\([A, B]\)

This generates another element in the algebra.

This satisifies:

\begin{itemize}
\item Bilinearity: \([xA+yB,C]=x[A,C]+y[B,C]\)
\item Alternativity: \([A,A]=0\)
\item Jacobi identity: \([A, [B,C]]+[C,[A,B]]+[B,[C,A]]=0\)
\item Anticommutivity: \([A, B]=-[B,A]\)
\end{itemize}

One option for the Lie bracket is the ring commutor. So that:

\([A,B]=AB-BA\)

