
\subsection{Solving quadratic polynomials}

\subsubsection{Quadratic polynomials}

Quadratic polynomials are of the form \(ax^2+bx+c=0\).

\subsubsection{Solving quadratic polynomials}

\(x=\frac{-b\pm \sqrt {b^2-4ac}}{2a}\)

\subsubsection{Proof}

We can get the two solutions to a quadratic equation from the following manipulation.

\(ax^2+bx+c=0\)

\(a[x^2+\frac{b}{a}x]=-c\)

\(a[(x+\frac{b}{2a})^2-\frac{b^2}{4a^2}]=-c\)

\(a[(x+\frac{b}{2a})^2]=\frac{b^2}{4a}-c\)

\((x+\frac{b}{2a})^2=\frac{b^2-4ac}{4a^2}\)

\(x+\frac{b}{2a}=\pm \sqrt {\frac{b^2-4ac}{4a^2}}\)

\(x=\frac{-b\pm \sqrt {b^2-4ac}}{2a}\)

