
\subsection{The chain rule, the product rule and the quotient rule}

\subsubsection{Chain rule}

$f(x)=f(g(x))$

$\frac{\delta f}{\delta x}=\lim_{\epsilon \rightarrow 0^+}\frac{f(g(x+\epsilon) )-f(g(x))}{\epsilon }$

$\frac{\delta f}{\delta x}=\lim_{\epsilon \rightarrow 0^+}\frac{g(x+\epsilon )-g(x)}{g(x+\epsilon )-g(x)}\frac{f(g(x+\epsilon) )-f(g(x))}{\epsilon }$

$\frac{\delta f}{\delta x}=\lim_{\epsilon \rightarrow 0^+}\frac{g(x+\epsilon )-g(x)}{\epsilon }\frac{f(g(x+\epsilon) )-f(g(x))}{g(x+\epsilon )-g(x)}$

$\frac{\delta f}{\delta x}=\lim_{\epsilon \rightarrow 0^+}[\frac{g(x+\epsilon )-g(x)}{\epsilon }]\lim_{\epsilon \rightarrow 0^+}[\frac{f(g(x+\epsilon) )-f(g(x))}{g(x+\epsilon )-g(x)}]$

$\frac{\delta f}{\delta x}=\frac{\delta g}{\delta x}\frac{\delta f}{\delta g}$

\subsubsection{Product rule}

$y=f(x)g(x)$

$\frac{\delta y}{\delta x}=\lim_{\epsilon \rightarrow 0^+}\frac{f(x+\epsilon )g(x+\epsilon )-f(x)g(x)}{\epsilon }$

$\frac{\delta y}{\delta x}=\lim_{\epsilon \rightarrow 0^+}\frac{f(x+\epsilon )g(x+\epsilon )-f(x)g(x+\epsilon )+f(x)g(x+\epsilon )-f(x)g(x)}{\epsilon }$

$\frac{\delta y}{\delta x}=\lim_{\epsilon \rightarrow 0^+}\frac{f(x+\epsilon )g(x+\epsilon )-f(x)g(x+\epsilon )}{\epsilon }+\lim_{\epsilon \rightarrow 0^+}\frac{f(x)g(x+\epsilon )-f(x)g(x)}{\epsilon }$

$\frac{\delta y}{\delta x}=\lim_{\epsilon \rightarrow 0^+}g(x+\epsilon )\frac{f(x+\epsilon )-f(x)}{\epsilon }+\lim_{\epsilon \rightarrow 0^+}f(x)\frac{g(x+\epsilon )-g(x)}{\epsilon }$

$\frac{\delta y}{\delta x}=g(x)\frac{\delta f}{\delta x }+f(x)\frac{\delta g}{\delta x}$

\subsubsection{Quotient rule}

$y=\frac{f(x)}{g(x)}$

$\frac{\delta }{\delta x}y=\frac{\delta }{\delta x}\frac{f(x)}{g(x)}$

$\frac{\delta }{\delta x}y=\frac{\delta }{\delta x}f(x)\frac{1}{g(x)}$

$\frac{\delta }{\delta x}y=\frac{\delta f}{\delta x}\frac{1}{g(x)}-\frac{\delta g}{\delta x}\frac{f(x)}{g(x)^2}$

$\frac{\delta }{\delta x}y=\frac{\frac{\delta f}{\delta x}g(x)-\frac{\delta g}{\delta x}f(x)}{g(x)^2}$

