
\subsection{Differentiating \(e^x\)}

\subsubsection{Intro}

We have \(e^x=\sum^{\infty }_{i=0} \frac{x^i}{i!}\)

\(\frac{\delta }{\delta x}e^x=\frac{\delta }{\delta x}\sum^{\infty }_{i=0} \frac{x^i}{i!}\)

\(\frac{\delta }{\delta x}e^x=\sum^{\infty }_{i=0} \frac{\delta }{\delta x}\frac{x^i}{i!}\)

\(\frac{\delta }{\delta x}e^x=\sum^{\infty }_{i=1} \frac{\delta }{\delta x}\frac{x^i}{i!}\)

\(\frac{\delta }{\delta x}e^x=\sum^{\infty }_{i=1} \frac{x^{i-1}}{(i-1)!}\)

\(\frac{\delta }{\delta x}e^x=\sum^{\infty }_{i=0} \frac{x^{i}}{i!}\)

\(\frac{\delta }{\delta x}e^x=e^x\)

