
\subsection{Integration by parts}

\subsubsection{Integration by parts}

We have:

$\frac{\delta y}{\delta x}=f(x)g(x)$

We want that in terms of \(y\).

We know from the product rule of differentiation:

$y=a(x)b(x)$

Means that:

$\frac{\delta y}{\delta x}=a'(x)b(x)+a(x)b'(x)$

So let's relabel \(f(x)\) as \(h'(x)\)

$\delta$

$\frac{\delta y}{\delta x}=h'(x)g(x)$

$\frac{\delta y}{\delta x}+h(x)g'(x)=h'(x)g(x)+h(x)g'(x)$

$y+\int h(x)g'(x)=\int h'(x)g(x)+h(x)g'(x)$

$y+\int h(x)g'(x)=h(x)g(x)$

$y=h(x)g(x)-\int h(x)g'(x)$

For example:

$\frac{\delta y}{\delta x}=x.\cos(x)$

$f(x)=cos(x)$

$g(x)=x$

$h(x)=sin(x)$

$g'(x)=1$

So:

$y=x\int cos(x) dx-\int sin(x)dx$

$y=xsin(x)-cos(x)+c$

