
\subsection{Symmetric and antisymmetric tensors}

Consider a tensor, e g \(T_{abc}\).

In general, this is not symmetric, that is:

\(T_{abc}\ne T_{bac}\)

\subsubsection{Symmetric part of a tensor}

We can write the symmetric part of this with regard to \(a\) and \(b\).

\(T_{(ab)c}=\dfrac{1}{2}(T_{abc}+T_{bac})\)

Clearly, \(T_{(ab)c}=T_{(ba)c}\)

\subsubsection{Antisymmetric part of a tensor}

We can also have an an antisymmetric part with regard to \(a\) and \(b\).

\(T_{[ab]c}=\dfrac{1}{2}(T_{abc}-T_{bac})\)

Clearly, \(T_{[ab]c}=-T_{[ba]c}\)

\subsubsection{Tensors as sums of their symmetric and antisymmetric parts}

\(T_{(ab)c}+T_{[ab]c}=\dfrac{1}{2}(T_{abc}+T_{bac})+\dfrac{1}{2}(T_{abc}-T_{bac})\)

\(T_{(ab)c}+T_{[ab]c}=T_{abc}\)

