
\subsection{The Robinson estimator}

\subsubsection{Partialling out}

\(y_i=\mathbf x_i\theta +g(\mathbf z_i) +\epsilon_i\)

Consider:

\(E(y_i|\mathbf z_i)=E(\mathbf x_i\theta +g(\mathbf z_i) + \epsilon_i|\mathbf z_i)\)

\(E(y_i|\mathbf z_i)=E(\mathbf x_i\theta|\mathbf z_i)+E(g(\mathbf z_i)|\mathbf z_i) + E(\epsilon_i|\mathbf z_i)\)

\(E(y_i|\mathbf z_i)=E(\mathbf x_i|\mathbf z_i)\theta+g(\mathbf z_i)\)

We can now remove the parametric part:

\(y_i-E(y_i|\mathbf z_i)=\mathbf x_i\theta +g(\mathbf z_i) + \epsilon_i - E(\mathbf x_i|\mathbf z_i)\theta -g(\mathbf z_i)\)

\(y_i-E(y_i|\mathbf z_i)=(\mathbf x_i- E(\mathbf x_i|\mathbf z_i))\theta +\epsilon_i\)

We define:

\begin{itemize}
\item \(\bar y_i = y_i-E(y_i|\mathbf z_i)\)
\item \(\bar x_i = \mathbf x_i- E(\mathbf x_i|\mathbf z_i)\)
\end{itemize}

\(\bar y_i =\bar x_i \theta +\epsilon_i\)

\subsubsection{Estimating \(\bar y_i\) and \(\bar x_i\)}

So we can use OLS if we can estimate.

\begin{itemize}
\item \(E(y_i|\mathbf z_i)\)
\item \(E(\mathbf x_i|\mathbf z_i)\)
\end{itemize}

We can do this with non-parametric methods.

