
\subsection{First-order conditions}

We have a utility function:

\(U=f(\mathbf x)\)

And the constraint:

\(\sum_i (x_i-c_i)p_i\le 0\)

This gives us the constrained optimisation problem:

\(L=f(\mathbf x)-\lambda \sum_i (x_i-c_i)p_i\)

The first-order conditions are:

\(L_{x_i}=\dfrac{\delta }{\delta x_i}f(\mathbf x)-\lambda p_i=0\)

Or:

\(\lambda = \dfrac{MU(x_i)}{p_i}\)

This means for any pair we have:

\(\dfrac{MU(x_i)}{p_i}=\dfrac{MU(x_j)}{p_j}\)

For the Cobb-Douglas utility function the first-order conditions are:

\(\dfrac{\delta }{\delta x_1}f(\mathbf x) = \dfrac{1}{x_1}\alpha_1\prod_i x_i^{\alpha_i}\)

\(L_{x_i}=\dfrac{\delta }{\delta x_i}f(\mathbf x)-\lambda p_i=0\)
