
\subsection{Kernel regression}

\subsubsection{Introduction}

For parametric regression we have:

\(y=f(X)\)

Where the form of \(f(X)\) is fixed, such as for linear regression.

For non-parametric regression we have:

\(y=m(X)\)

Where \m(X)\) is not fixed.

We can estimate \(m(X)\) using kernel regression.

\(m(X)=\frac{\sum_{i=1}^nK_h(x-x_i)y_i}{\sum_{i=1}^nK_h(x-x_i)}\)

We know this because we have:

\(E(y|X)=\int yf(y|x)dy=\int y\frac{f(x,y)}{f(x)}dy\)

We then use kernel density estimation for both.

