
\subsection{Single equality constraint}

\subsubsection{Constrained optimisation}

Rather than maximise \(f(x)\), we want to maximise \(f(x)\) subject to \(g(x)=0\).

We write this, the Lagrangian, as:

$\mathcal{L}(x,\lambda )=f(x)-\sum^m_k\lambda_k [g_k(x)-c_k]$

We examine the stationary points for both vector \(x\) and \(\lambda \). By including the latter we ensure that these points are consistent with the constraints.

\subsubsection{Solving the Langrangian with one constraint}

Our function is:

$\mathcal{L}(x, \lambda )=f(x)-\lambda [g(x)-c]$

The first-order conditions are:

$\mathcal{L}_{\lambda }= -[g(x)-c]$

$\mathcal{L}_{x_i}=\frac{\delta f}{\delta x_i}-\lambda \frac{\delta g}{\delta x_i}$

The solution is stationary so:

$\mathcal{L}_{x_i}=\frac{\delta f}{\delta x_i}-\lambda \frac{\delta g}{\delta x_i}=0$

$\lambda \frac{\delta g}{\delta x_i}=\frac{\delta f}{\delta x_i}$

$\lambda =\frac{\frac{\delta f}{\delta x_i}}{\frac{\delta g}{\delta x_i}}$

Finally, we can use the following in practical applications.

$\frac{\frac{\delta f}{\delta x_i}}{\frac{\delta g}{\delta x_i}}=\frac{\frac{\delta f}{\delta x_j}}{\frac{\delta g}{\delta x_j}}$

