
\subsection{Variance of OLS estimators}

\subsubsection{Variance-covariance matrix}

We know:

\(\hat \theta =(X^TX)^{-1}X^Ty\)

\(y=X\theta +\epsilon\)

Therefore:

\(\hat \theta =(X^TX)^{-1}X^T(X\theta +\epsilon)\)

\(\hat \theta =\theta +(X^TX)^{-1}X^T\epsilon\)

\(\hat \theta -\theta =(X^TX)^{-1}X^T\epsilon\)

\(Var [\hat \theta ]=E[(\hat \theta -\theta)(\hat \theta -\theta )^T]\)

\(Var [\hat \theta ]=E[(X^TX)^{-1}X^T\epsilon(X^TX^{-1}X^T\epsilon )^T]\)

\(Var [\hat \theta ]=E[(X^TX)^{-1}X^T\epsilon \epsilon^T X(X^TX)^{-1}]\)

\(Var [\hat \theta ]=(X^TX)^{-1}X^TE[\epsilon \epsilon^T ]X(X^TX)^{-1}\)

We write:

\(\Omega=E[\epsilon \epsilon^T]\)

\(Var [\hat \theta ]=(X^TX)^{-1}X^T\Omega X(X^TX)^{-1}\)

Depending on how we estimate \(\Omega\), we get different variance terms.

\subsubsection{Variance under IID}

If IID:

\(\Omega = I\sigma^2_{\epsilon }\)

\(Var [\hat \theta ]=(X^TX)^{-1}X^TI\sigma^2_{\epsilon } X(X^TX)^{-1}\)

\(Var [\hat \theta ]=\sigma^2_\epsilon (X^TX)^{-1}\)

