\subsection{Partial fraction decomposition}

We have:
$\frac{1}{A.B}$

We want this in the form of:

$\frac{a}{A}+\frac{b}{B}$

First, lets define \(M\) as the mean of these two numbers, and define \(\delta=M-B\). Then:

$\frac{1}{AB}=\frac{1}{(M+\delta)(M-\delta)}=\frac{a}{M+\delta}+\frac{b}{M-\delta}$

We can rearrange the latter two to find:

$1=a(M-\delta)+b(M+\delta)$

Now we need to find values of \(a\) and \(b\) to choose.

Let's examine \(a\).

$a=\frac{1-b(M+\delta)}{M-\delta}$

$a=-\frac{bM+b\delta -1}{M-\delta}$

$a=-\frac{bM+b\delta -1}{M-\delta}$

For this to divide neatly we need both the numerator to be a constant multiplier of the denominator. This means the ratio the multiplier for the left hand side of the denominator is equal to the right:

$\frac{bM}{M}=\frac{b\delta -1}{-\delta}$

$b=\frac{b\delta -1}{-\delta}$

$b=\frac{1}{2\delta}$

We can do the same for \(a\).

$a=-\frac{1}{2\delta}$

We can plug these back into our original formula:

$\frac{1}{(M+\delta)(M-\delta)}=\frac{-\frac{1}{2\delta}}{M+\delta}+\frac{\frac{1}{2\delta}}{M-\delta}$

$\frac{1}{(M+\delta)(M-\delta)}=\frac{1}{2\delta}[\frac{1}{M-\delta}-\frac{1}{M+\delta}]$

