
\subsection{Addition of sine and cosine}

\subsubsection{Adding waves with same frequency}

We know that:

\(a\sin(bx+c)=a\sin(bx)\cos(c)+a\sin(c)\cos(bx)\)

So:

\(a\sin(bx+c)+d\sin(bx+e)=a\sin(bx)\cos(c)+a\sin(c)\cos(bx)+ d\sin(bx)\cos(e)+d\sin(e)\cos(bx)\)

We know that:

\(\sin(\theta )=\frac{e^{i\theta }-e^{-i\theta }}{2i}\)

So:

\(a\sin(bx+c)+d\sin(bx+f)=a\frac{e^{i(bx+c)}-e^{-i(bx+c)}}{2i}+d\frac{e^{i(bx+f)}-e^{-i(bx+f)}}{2i}\)

\(a\sin(bx+c)+d\sin(bx+f)=\frac{a(e^{i(bx+c)}-e^{-i(bx+c)})+d(e^{i(bx+f)}-e^{-i(bx+f)})}{2i}\)

\(a\sin(bx+c)+d\sin(bx+f)=\frac{a(e^{ibx}e^{ic}-e^{-ibx}e^{-ic})+d(e^{ibx}e^{if}-e^{-ibx}e^{-if)})}{2i}\)

\(a\sin(bx+c)+d\sin(bx+f)=\frac{(e^{ibx}(ae^{ic}+de^{if})-e^{-ibx}(ae^{-c}+d^{-if})}{2i}\)

\(a_i\sin(b_ix+c_i)+a_j\sin(b_jx+c_j)=a_i\sin(b_ix+c_i)+a_j\sin(b_ix+c_j)\)

\(a_i\sin(b_ix+c_i)+a_j\sin(b_jx+c_j)=a_i\sin(b_ix)\cos(c_i)+a_i\sin(c_i)\cos(b_ix)+a_j\sin(b_ix)\cos(c_j)+a_j\sin(c_j)\cos(b_ix)\)

