
\subsection{Mean Squared Error (MSE) and Root Mean Squared Error (RMSE) of an estimator}

\subsubsection{Mean squared error}

Mean squared error

\(MSE = E[(\hat \theta - \theta )^2]=E[((\hat \theta - E[\hat \theta ])+(E[\hat \theta ]-\theta ))^2]\)

\(MSE = E[(\hat \theta - \theta )^2]=E[(\hat \theta - E[\hat \theta ])^2+(E[\hat \theta ]-\theta )^2+2(E[\hat \theta ]-\theta )(\hat \theta- E[\hat \theta ])]\)

\(MSE = E[(\hat \theta - \theta )^2]=E[(\hat \theta - E[\hat \theta ])^2]+E[(E[\hat \theta ]-\theta)^2] +E[2(E[\hat \theta ]-\theta )(\hat \theta- E[\hat \theta ])]\)

\(MSE = E[(\hat \theta - \theta )^2]=Var(\hat \theta )+(E[\hat \theta ]-\theta)^2 +2(E[\hat \theta ]-\theta )E[\hat \theta- E[\hat \theta ]]\)

\(MSE = E[(\hat \theta - \theta )^2]=Var(\hat \theta )+Bias (\hat \theta )^2\)

\subsubsection{Root Mean Square Error (RMSE)}

This is the square root of the MSE.

It is also called the Root Mean Square Deviation (RMSD)

