
\subsection{Introduction}
\begin{verbatim}
L = T-V
T = \sum_i^n(1/2)m_iv_i^2
V=G\sum_i^{n-1}\sum_{i+1}^n\frac{m_im_j}{|\bold{r}_i-\bold{r}_j|}
\end{verbatim}
\subsection{euler lagrange}
\begin{verbatim}
\dfrac{d}{dt}(\dfrac{\delta L}{\delta \bold{r}^{dot}_i})-\dfrac{\delta L}{\delta \bold{r}_i}=0
\dfrac{\delta L}{\delta \bold{r}^{dot}_i}=m_i\bold{r}^{dot}_i=\bold{p}_i
\dfrac{\delta L}{\delta \bold{r}_i}=-G\sum_{j=1,j\ne i}^nm_im_j\dfrac{\bold{r}_i-\bold{r}_j}{|\bold{r}_i-\bold{r}_j|^3}
\end{verbatim}

gives us
\begin{verbatim}
m_i\bold{r}^{dot dot}_i=-G\sum_{j=1,j\ne i}^nm_im_j\dfrac{\bold{r}_i-\bold{r}_j}{|r_i-r_j|^3}
\end{verbatim}
which is
\begin{verbatim}
~ ma=F
\end{verbatim}
also gives
\begin{verbatim}
\bold{r}^{dot dot}_i=-G\sum_{j=1,j\ne i}^nm_j\dfrac{\bold{r}_i-\bold{r}_j}{|r_i-r_j|^3}

\end{verbatim}

