
\subsection{Even and odd functions}

\subsubsection{Defining odd and even functions}

An even function is one where:

\(f(x)=f(-x)\)

An odd function is one where:

\(f(x)=-f(-x)\)

\subsubsection{Functions which are even and odd}

If a function is even and odd:

\(f(x)=f(-x)=-f(-x)\)

\(f(x)=-f(x)\)

Then \(f(x)=0\).
\subsubsection{Scaling odd and even functions}

Scaling an even function provides an even function.

\(h(x)=c.f(x)\)

\(h(-x)=c.f(-x)\)

\(h(-x)=c.f(x)\)

\(h(-x)=h(x)\)

Scaling an odd function provides an odd function.

\(h(x)=c.f(x)\)

\(-h(-x)=-c.f(-x)\)

\(-h(-x)=c.f(x)\)

\(-h(-x)=h(x)\)

\subsubsection{Adding odd and even functions}

Note than \(2\) even functions added together makes an even function.

\(h(x)=f(x)+g(x)\)

\(h(x)=f(-x)+g(-x)\)

\(h(-x)=f(x)+g(x)\)

\(h(x)=h(-x)\)

And adding \(2\) odd functions together makes an odd function.

\(h(x)=f(x)+g(x)\)

\(h(x)=-f(-x)-g(-x)\)

\(-h(-x)=f(x)+g(x)\)

\(-h(-x)=h(x)\)

\subsubsection{Multiplying odd and even functions}

Multiplying \(2\) even functions together makes an even function.

\(h(x)=f(x)g(x)\)

\(h(-x)=f(-x)g(-x)\)

\(h(-x)=f(x)g(x)\)

\(h(-x)=h(x)\)

Multiplying \(2\) odd functions together makes an even function.

\(h(x)=f(x)g(x)\)

\(h(-x)=f(-x)g(-x)\)

\(h(-x)=(-1).(-1.)f(x)g(x)\)

\(h(-x)=h(x)\)

