
\subsection{Integration by parts}

We have:

\(\dfrac{\delta y}{\delta x}=f(x)g(x)\)

We want that in terms of \(y\).

We know from the product rule of differentiation:

\(y=a(x)b(x)\)

Means that:

\(\dfrac{\delta y}{\delta x}=a'(x)b(x)+a(x)b'(x)\)

So let's relabel \(f(x)\) as \(h'(x)\)

\(\delta\)

\(\dfrac{\delta y}{\delta x}=h'(x)g(x)\)

\(\dfrac{\delta y}{\delta x}+h(x)g'(x)=h'(x)g(x)+h(x)g'(x)\)

\(y+\int h(x)g'(x)=\int h'(x)g(x)+h(x)g'(x)\)

\(y+\int h(x)g'(x)=h(x)g(x)\)

\(y=h(x)g(x)-\int h(x)g'(x)\)

For example:

\(\dfrac{\delta y}{\delta x}=x.\cos(x)\)

\(f(x)=\cos(x)\)

\(g(x)=x\)

\(h(x)=\sin(x)\)

\(g'(x)=1\)

So:

\(y=x\int \cos(x) dx-\int \sin(x)dx\)

\(y=x\sin(x)-\cos(x)+c\)

