
\subsection{Solving quadratic polynomials}

\subsubsection{Quadratic polynomials}

Quadratic polynomials are of the form \(ax^2+bx+c=0\).

\subsubsection{Solving quadratic polynomials}

\(x=\dfrac{-b\pm \sqrt {b^2-4ac}}{2a}\)

\subsubsection{Proof}

We can get the two solutions to a quadratic equation from the following manipulation.

\(ax^2+bx+c=0\)

\(a[x^2+\dfrac{b}{a}x]=-c\)

\(a[(x+\dfrac{b}{2a})^2-\dfrac{b^2}{4a^2}]=-c\)

\(a[(x+\dfrac{b}{2a})^2]=\dfrac{b^2}{4a}-c\)

\((x+\dfrac{b}{2a})^2=\dfrac{b^2-4ac}{4a^2}\)

\(x+\dfrac{b}{2a}=\pm \sqrt {\dfrac{b^2-4ac}{4a^2}}\)

\(x=\dfrac{-b\pm \sqrt {b^2-4ac}}{2a}\)

