
\subsection{Lagrangians}

We have:

\(S = \int_a^b \sqrt {(\mathbf {\dot q})^T\mathbf M\mathbf {\dot q}}dt\)

We can define:

\(L=\sqrt {(\mathbf {\dot q})^T\mathbf M\mathbf {\dot q}}\)

So we have:

\(S=\int_a^b L dt\)

\subsection{Principle of stationary action}

\(\delta A=0\)

That is, the coordinates and their velocities are such that action is stationary.

\subsection{Euler-Lagrange}

We have \(q(t)\) which makes the action stationary. Consider adding proportion \(\epsilon \) of another function \(f(t)\) to \(q(t)\).

\(A’=\int_{t_0}^{t_1} L[q(t)+\epsilon f(t), \dot {q(t)}+\epsilon f’(t)]dt\)

\(\dfrac{A’-A}{\epsilon }=\dfrac{1}{\epsilon}\int_{t_0}^{t_1} L[q(t)+\epsilon f(t), \dot {q(t)}+\epsilon f’(t)]-L[q,\dot q]dt\)

We can do a Taylor expansion of \(A’\).

\(A’=\int_{t_0}^{t_1} L[q(t)+\epsilon f(t), \dot {q(t)}+\epsilon f’(t)]dt\)

\(A’=\int_{t_0}^{t_1} L[q(t),\dot {q(t)}]+\epsilon [f\dfrac{\delta L}{\delta q}+f^.\dfrac{\delta L}{\delta \dot q}]+\epsilon^2 [...]dt\)

So:

\(\dfrac{A’-A}{\epsilon }=\dfrac{1}{\epsilon}\int_{t_0}^{t_1}L[q(t),\dot {q(t)}]+\epsilon [f\dfrac{\delta L}{\delta q}+f^.\dfrac{\delta L}{\delta q^.}]+\epsilon^2 [...]-L[q,\dot q]dt\)

\(\dfrac{A’-A}{\epsilon }=\int_{t_0}^{t_1}[f\dfrac{\delta L}{\delta q}+f^.\dfrac{\delta L}{\delta \dot {q}}]+\epsilon [...]dt\)

We can now make the left side \(0\), by using the definition of stationary action.

\(\lim_{\epsilon \rightarrow 0} \dfrac{A’-A}{\epsilon }=\int_{t_0}^{t_1}[f\dfrac{\delta L}{\delta q}+f^.\dfrac{\delta L}{\delta \dot q}]dt\)

\(\int_{t_0}^{t_1}[f\dfrac{\delta L}{\delta q}+f^.\dfrac{\delta L}{\delta \dot q}]dt=0\)

\(\int_{t_0}^{t_1}[f\dfrac{\delta L}{\delta q}]dt +\int_{t_0}^{t_1}[f^.\dfrac{\delta L}{\delta \dot q}]dt=0\)

Note that

\(\int_{t_0}^{t_1}[f^.\dfrac{\delta L}{\delta \dot q}]dt=[f\dfrac{\delta L}{\delta \dot q}]_{t_0}^{t_1}-\int_{t_0}^{t_1}f \dfrac{d}{dt}\dfrac{\delta L}{\delta \dot q}dt\)

We assume that \(f(t_0)=f(t_1)=0\) and so:

\(\int_{t_0}^{t_1}[f^.\dfrac{\delta L}{\delta \dot q}]dt=-\int_{t_0}^{t_1}f \dfrac{d}{dt}\dfrac{\delta L}{\delta \dot q}dt\)

Plugging this back in we get:

\(\int_{t_0}^{t_1}[f\dfrac{\delta L}{\delta q}]-f \dfrac{d}{dt}\dfrac{\delta L}{\delta \dot q}dt]=0\)

\(\int_{t_0}^{t_1}f[\dfrac{\delta L}{\delta q}]-\dfrac{d}{dt}\dfrac{\delta L}{\delta \dot q}dt]=0\)

Since this applies to all possible functions we get:

\(\dfrac{\delta L}{\delta q}=\dfrac{d}{dt}\dfrac{\delta L}{\delta \dot q}\)

\subsection{Definition: Momentum}

\(p=\dfrac{\delta L}{\delta \dot q}\)

\subsection{EL v2}
\(L=\sqrt {(\mathbf {\dot q})^T\mathbf M\mathbf {\dot q}}\)

\(\dfrac{\delta L}{\delta q}- \dfrac{d}{dt}(\dfrac{\delta L}{\delta \dot q})=0\)

We have

\(S=\int_a^b L(q(t), \dot q(t))dt \)

\(\delta S=\delta \int_a^b L(q(t), \dot q(t))dt \)

\(J=\int_a^b L(t,q(t), \dot q(t)) dt\)

\(J=\sum_{k=0}^{n-1}\)


\subsection{EL v3}


\(A=\sum L(x(t), \dot x(t)) \delta t \)

\(A=\sum L(\dfrac{x(t)+x(t-1)}{2}, \dfrac{x(t)-x(t-1)}{\delta t}) \delta t \)

 

\(\dfrac{\delta }{\delta x(t)}A = \sum \dfrac{\delta }{\delta x(t)}L(\dfrac{x(t)+x(t-1)}{2}, \dfrac{x(t)-x(t-1)}{\delta t}) \delta t \)

 

\(\dfrac{\delta }{\delta x(t)}A = \delta t [\dfrac{\delta }{\delta x(t)}L(\dfrac{x(t)+x(t-1)}{2}, \dfrac{x(t)-x(t-1)}{\delta t}) + \dfrac{\delta }{\delta x(t)}L(\dfrac{x(t+1)+x(t)}{2}, \dfrac{x(t+1)-x(t)}{\delta t})]\)

 

\(\dfrac{\delta }{\delta x(t)}A = \delta t [\dfrac{1}{2}L_x +\dfrac{1}{\delta t}L_{\dot x} + \dfrac{1}{2}L_x -\dfrac{1}{\delta t}L_{\dot x}]\)

 

\(A=\int_a^b L(q(t), \dot q(t)) dt\)

\(A=\sum L(q(t), \dot q(t)) \delta t\)

\(A=\sum L(\dfrac{q(t)+q(t-1)}{2}, \dfrac{q(t)-q(t-1)}{\delta t}) \delta t\)

\(\dfrac{\delta }{\delta q_i(t)}A = \sum \dfrac{\delta }{\delta q_i(t)}L(\dfrac{q(t)-q(t-1)}{2}, \dfrac{q(t)-q(t-1)}{\delta t}) \delta t\)

\(\dfrac{\delta }{\delta q_i(t)}A = \delta t [\dfrac{\delta }{\delta q_i(t)}L(\dfrac{q(t)+q(t-1)}{2}, \dfrac{q(t)-q(t-1)}{\delta t})+\dfrac{\delta }{\delta q_i(t)}L(\dfrac{q(t+1)+q(t)}{2}, \dfrac{q(t+1)-q(t)}{\delta t})]\)

 

\(\dfrac{\delta }{\delta q_i(t)}A = \delta t [\dfrac{1}{2}L_{q_i}+\dfrac{1}{\delta t}L_{\dot q_i}+\dfrac{1}{2}L_{q_i}-\dfrac{1}{\delta t}L_{\dot q_i}+\dfrac{\delta }{\delta q_i(t)}L(\dfrac{q(t+1)+q(t)}{2}, \dfrac{q(t+1)-q(t)}{\delta t})]\)

