
\subsection{Outcome}


\(\dfrac{\delta L}{\delta q}=\dfrac{d}{dt}\dfrac{\delta L}{\delta \dot q}\)


\(L=\sqrt {(\mathbf {\dot q})^T\mathbf M\mathbf {\dot q}}\)

If \(M=I\), then:

\(L=\sqrt {(\mathbf {\dot q})^T \mathbf {\dot q}}\)

In 1 dimension, Euclid:

\(L=\sqrt {\dot q^2}\)
\(L=\dot q\)


So:

\(\dfrac{\delta L}{\delta q}=\dfrac{\delta }{\delta q}\dot q\)
\(\dfrac{\delta L}{\delta q}=0\)

\(\dfrac{\delta L}{\delta \dot q}=\dfrac{\delta }{\delta \dot q}\dot q\)
\(\dfrac{\delta L}{\delta \dot q}=1\)

Into Euler-Lagrange:

\(\dfrac{\delta L}{\delta q}=\dfrac{d}{dt}\dfrac{\delta L}{\delta \dot q}\)
\(0=\dfrac{d}{dt}1\)


In three dimensions:

\(L=\sqrt {\dot x^2 + \dot y^2 + \dot z^2}\)

So:

\(\dfrac{\delta L}{\delta q}=\dfrac{\delta }{\delta q}\sqrt {\dot x^2 + \dot y^2 + \dot z^2}\)
\(\dfrac{\delta L}{\delta q}=0\)

\(\dfrac{\delta L}{\delta \dot q}=\dfrac{\delta }{\delta \dot q}\sqrt {\dot x^2 + \dot y^2 + \dot z^2}\)

